theories/clang/lib/list.v
@@ -6,51 +6,86 @@ Require Import lib.gmap_solve.
 Section proof.
   Context `{clangG Σ}.
 
-  Fixpoint isList (l: val) (xs: list val) (t: type) :=
-    match xs with
-      | [] => (⌜ l = null ⌝)%I
-      | x::xs' => (∃ p l',
-                     ⌜ l = Vptr p ∧ typeof t x ⌝ ∗
-                     p ↦ Vpair x l' @ (Tprod t (Tptr t)) ∗ isList l' xs' t)%I
-    end.
-
-  Parameter y t px: addr.
-  Parameter x: ident.
-
   (* de brujin with autosubst? *)
   Definition tcell (telem: type): type := Tmu 0 (Tprod telem (Tptr (Tvar 0))).
   Definition tlist (telem: type): type := Tptr (tcell telem).
 
-  Definition rev_list (telem: type) : stmts :=
-    y <- null ;;
-    while [ x != null ] ( x != null ) <{
-      t <- snd (!x) ;;
-      snd (!x) <- !y ;;
-      y <- x ;;
-      x <- !t
-    }>;;
-    x <- !y.
+  Fixpoint isList (l: val) (xs: list val) (t: type) :=
+    match xs with
+      | [] => (⌜ l = null ⌝)%I
+      | x::xs' => (∃ p l',
+                     ⌜ l = Vptr p ∧ typeof t x ∧ typeof (tlist t) l' ⌝ ∗
+                     p ↦ Vpair x l' @ (Tprod t (Tptr t)) ∗ isList l' xs' t)%I
+    end.
 
-  Lemma rev_spec l ety Φ Φret body xs:
-    instantiate_f_body {[ x := (tlist ety, px) ]} (rev_list ety) = Some body →
-    isList l xs ety ∗ y ↦ - ∗ t ↦ - ∗ px ↦ l @ tlist ety ∗
-    (isList l (rev xs) ety -∗ Φ Vvoid)
+  Parameter py pt px: addr.
+  Parameter x: ident.
+
+  Definition rev_list (telem: type) : stmts :=
+    while [ x != null ] ( x != null ) <{
+      pt <- snd (!x) ;;
+      snd (!x) <- !py ;;
+      py <- x ;;
+      x <- !pt
+    }>.
+
+  Lemma rev_spec Φ Φret body xs:
+    ∀ lx ly ys,
+    instantiate_f_body {[ x := (tlist Tint32, px) ]} (rev_list Tint32) = Some body →
+    isList lx xs Tint32 ∗ isList ly ys Tint32 ∗ pt ↦ - ∗
+    px ↦ lx @ tlist Tint32 ∗ py ↦ ly @ tlist Tint32 ∗
+    (∀ ly', py ↦ ly' @ tlist Tint32 ∗ isList ly' (rev xs ++ ys) Tint32 -∗ Φ Vvoid)
     ⊢ WP curs body {{ Φ; Φret }}.
   Proof.
     induction xs as [|x xs' IHxs'].
-    - iIntros (?) "(% & Hy & Ht & Hpx & HΦ)".
+    - iIntros (????) "(% & Hlr & Ht & Hpx & Hpy & HΦ)".
+      subst. rewrite /instantiate_f_body /resolve_rhs map_to_list_singleton in H0.
+      simpl in H0.
+      destruct (decide (x = x))=>//.
+      destruct px. gmap_solve.
+      wp_load. wp_op. simpl.
+      iApply wp_while_false.
+      iNext. iApply "HΦ". iFrame.
+    - iIntros (????) "(Hl & Hlr & Ht & Hpx & Hpy & HΦ)".
       rewrite /instantiate_f_body /resolve_rhs map_to_list_singleton in H0.
       simpl in H0.
       destruct (decide (x = x))=>//.
       destruct px. gmap_solve.
-      iDestruct "Hy" as (??) "Hy".
-      wp_assign. wp_load.
-      wp_op. simpl.
-      iApply wp_while_false.
-      iNext. wp_load. wp_assign.
-      by iApply "HΦ".
-    - 
-    
-    
+      wp_load. iDestruct "Hl" as (p l') "(% & Hp & Hl')".
+      destruct H0 as [? [? ?]]. subst.
+      wp_op. iApply wp_while_true.
+      iNext. repeat (iApply wp_seq).
+      iApply (wp_bind [EKderef; EKsnd] (SKassignl _)). (* TODO: Some bug in tactic *)
+      iApply wp_load. iFrame. iIntros "!> Hbo".
+      simpl. wp_load. wp_bind (Esnd _).
+      iApply wp_snd. iNext. iApply wp_value.
+      iDestruct "Ht" as (??) "Ht".
+      wp_assign. repeat (iApply wp_seq).
+      iApply (wp_bind [EKbinopr _ _] (SKassignr _)).
+      iApply wp_load. iFrame. iIntros "!> ?".
+      simpl. iApply (wp_bind [] (SKassignr _)).
+      destruct p as [pb po].
+      iApply wp_op=>//. simpl.
+      rewrite /offset_by_byte.
+      replace (Z.to_nat (Byte.intval (Byte.repr 4))) with 4%nat; last done.
+      wp_load. iApply (wp_assign_offset _ _ _ _ _ _ _ Tint32)=>//.
+      { admit. }
+      iFrame. iIntros "!> ?".
+      wp_load. iApply (wp_assign _ _ _ _ _ (tlist Tint32)).
+      apply typeof_ptr.
+      iFrame. iIntros "!> ?".
+      wp_load. iApply wp_assign.
+      { admit. }
+      iFrame. iIntros "!> ?".
+      iApply (IHxs' l' (Vptr (pb, po)) (x::ys)).
+      { rewrite /instantiate_f_body /resolve_rhs map_to_list_singleton.
+        simpl. destruct (decide (x = x))=>//.
+        destruct px. gmap_solve. done. }
+      iFrame. simpl.
+      iSplitL "~1 Hlr".
+      { iExists (pb, po), ly. iFrame. admit. }
+      iSplitL "Ht"; first eauto.
+      replace (rev xs' ++ x :: ys) with ((rev xs' ++ [x]) ++ ys); first done; last by rewrite -app_assoc.
+  Admitted.      
   
 End proof.
